\subsection{7.8}

(merk: subscript 2 fjernet for $\xi, A, amp$)
\begin{align}
	b_{22} &=  \frac{\bar{E}^{\infty} c_g + \bar{E}^{-\infty} c_g }{\frac{1}{2} |\xi|^2 \omega^2}\\
	b_{22} &=  \frac{\frac{1}{2}(\rho=1) g |amp^{\infty}|^2  c_g + \frac{1}{2}(\rho=1) g |amp^{-\infty}|^2 c_g }{\frac{1}{2} |\xi|^2 \omega^2}\\
	b_{22} &=  \frac{ g |amp^{\infty}|^2  (\frac{g}{2\omega}) +  g |amp^{-\infty}|^2 (\frac{g}{2\omega}) }{ |\xi|^2 \omega^2}\\
	b_{22} &=  \frac{ g {|\xi A^{\infty} \frac{\omega^2}{g}|}^2  (\frac{g}{2\omega}) +  g {|\xi A^{-\infty} \frac{\omega^2}{g}|}^2  (\frac{g}{2\omega}) }{ |\xi|^2 \omega^2}\\
b_{22} &=  \frac{  g \cancel{|\xi|^2} (\frac{\color{red}{\omega^2}}{g})(\frac{\omega^2}{g}) {| A^{\infty} |}^2  (\frac{g}{2\omega}) + g \cancel{|\xi|^2}  (\frac{\color{red}{\omega^2}}{g})(\frac{\omega^2}{g}) {| A^{-\infty}|}^2  (\frac{g}{2\omega}) }{ \cancel{|\xi|^2} \color{red}{\omega^2}}\\
b_{22} &=    \cancel{g  (\frac{1}{g})}(\frac{\omega^2}{g}) {| A^{\infty} |}^2  (\frac{g}{2\omega}) +  \cancel{g   (\frac{1}{g})}(\frac{\omega^2}{g}) {| A^{-\infty}|}^2  (\frac{g}{2\omega}) \\
b_{22} &=    (\frac{\omega^2}{g})   (\frac{g}{2\omega}) ({| A^{\infty} |}^2 +  {| A^{-\infty}|}^2)
\end{align}

